\documentclass{math}

\usepackage{tikz}
\usetikzlibrary{arrows.meta}

\title{Differential Equations}
\author{Alvin Lin}
\date{January 2018 - May 2018}

\begin{document}

\maketitle

\section*{Laplace Transforms}
Let \( f \) be a function defined on \( [0,\infty) \). The Laplace transform
of \( f \), \( \laplace{f(s)} \), is a function \( F(s) \), where \( s \)
is the new variable. The domain of \( \laplace{f} \), or \( F(s) \), is all
values of \( s \) for which the following converges:
\[ \laplace{f} = \int_{0}^{\infty}\e^{-st}f(t)\diff{t} \]
Recall the following:
\[ \int_{0}^{\infty}g(t)\diff{t} = \lim_{N\to\infty}\int_{0}^{N}g(t)\diff{t} \]
If this limit exists, it converges. Otherwise, it diverges.

\subsubsection*{Example}
Find \( \laplace{f(t)} \) where \( f(t) = 1 \).
\begin{align*}
  \laplace{1} &= \int_{0}^{\infty}\e^{-st}\diff{t} \\
  &= \lim_{N\to\infty}\int_{0}^{\infty}\e^{-st}\diff{t} \\
  &= \lim_{N\to\infty}\bigg[-\frac{1}{s}\e^{-st}\bigg]_{0}^{N} \\
  &= \lim_{N\to\infty}\bigg[-\frac{1}{\e^{sN}}-\bigg(-\frac{1}{s}\bigg)\bigg] \\
  &= \frac{1}{s}, \quad s > 0
\end{align*}
Additional fact: \( \laplace{0} = 0 \).

\subsubsection*{Example}
Find \( \laplace{\e^{at}} \) where \( a \) is real.
\begin{align*}
  f(t) &= \e^{at} \\
  \laplace{\e^{at}} &= \int_{0}^{\infty}\e^{-st}\e^{at}\diff{t} \\
  &= \int_{0}^{\infty}\e^{-(s-a)t}\diff{t} \\
  &= \lim_{N\to\infty}\int_{0}^{N}\e^{-(s-a)t}\diff{t} \\
  &= \lim_{N\to\infty}\bigg[-\frac{1}{s-a}\e^{-(s-a)t}\bigg]_{0}^{N} \\
  &= \lim_{N\to\infty}\bigg[-\frac{1}{s-a}\e^{-(s-a)N}-
    \bigg(-\frac{1}{s-a}\bigg)\bigg] \\
  &= \lim_{N\to\infty}-\frac{1}{s-a}\e^{-(s-a)N}+\frac{1}{s-a} \\
  &= \frac{1}{s-a}, \quad s-a > 0 \\
  &= \frac{1}{s-a}, \quad s>a \\
  \laplace{\e^{2t}} &= \frac{1}{s-2} \\
  \laplace{\e^{-2t}} &= \frac{1}{s+2}
\end{align*}

\subsubsection*{Example}
Find \( \laplace{t} \).
\begin{align*}
  f(t) &= t \\
  \laplace{t} &= \int_{0}^{\infty}t\e^{-st}\diff{t} \\
  &= \lim_{N\to\infty}\int_{0}^{N}t\e^{-st}\diff{t} \\
\end{align*}
\begin{align*}
  &= \lim_{N\to\infty}\bigg[-\frac{1}{s}\e^{-st}t\bigg]_{0}^{N}-
    \int_{0}^{N}-\frac{1}{s}\e^{-st}\diff{t} \\
  &= \lim_{N\to\infty}\bigg[
    -\frac{1}{s}\e^{-st}t+\frac{1}{s}(-\frac{1}{s}\e^{-st})\bigg]_{0}^{N}
  &= \lim_{N\to\infty}\bigg[
    (-\frac{1}{s}\e^{-sN}N)+(-\frac{1}{s^2}\e^{-sN}-\frac{1}{s^2})\bigg] \\
  &= \frac{1}{s^2}, \quad s>0
\end{align*}
As a general rule, for \( f(t) = t^n \) where \( n \) is a non-negative integer:
\begin{align*}
  \laplace{t^n} &= \frac{n!}{s^{n+1}} \\
  \laplace{t^3} &= \frac{3!}{s^{3+1}} = \frac{6}{s^4}
\end{align*}
Additionally, for sines and cosines:
\begin{align*}
  \laplace{\sin(bt)} &= \frac{b}{s^2+b^2}, \quad s>0,b\ne0 \\
  \laplace{\cos(bt)} &= \frac{s}{s^2+b^2}, \quad s>0,b\ne0 \\
  \laplace{\sin(\sqrt{2}t)} &= \frac{\sqrt{2}}{s^2+2} \\
  \laplace{\cos(\sqrt{2}t)} &= \frac{s}{s^2+2}
\end{align*}

\subsection*{Property of Linearity}
Given \( f(t),g(t) \) and \( k \) a constant:
\begin{enumerate}
  \item \( \laplace{f(t)\pm g(t)} = \laplace{f(t)}\pm\laplace{g(t)} \)
  \item \( \laplace{kf(t)} = k\laplace{f(t)} \)
\end{enumerate}

\subsubsection*{Example}
\[ \laplace{7+5\e^{-7t}-7\sin(3t)+7t^2+5\cos(7t)} \]
\begin{align*}
  &= \laplace{7}+\laplace{5\e^{-7t}}-\laplace{7\sin(3t)}+\laplace{7t^2}+
    \laplace{5\cos(7t)} \\
  &= 7\laplace{1}+5\laplace{\e^{-7t}}-7\laplace{\sin(3t)}+7\laplace{t^2}+
    5\laplace{\cos(7t)} \\
  &= \frac{7}{s}+\frac{5}{s+7}-\frac{(7)(3)}{s^2+9}+\frac{(7)(2!)}{s^3}+
    \frac{5s}{s^2+49}, \quad s>0
\end{align*}
Note that each term has a different condition for \( s \), so we need to take
the intersection of the conditions.

\subsection*{Existence of the Transform}
Consider a piecewise continuous function \( f \) over \( [a,b] \). \( f \) has
a finite number of jump discontinuities.
\begin{center}
  \begin{tikzpicture}[shorten >=-2pt,shorten <=-2pt]
    \draw[->,very thick] (0,0) -- (5,0);
    \draw[->,very thick] (0,0) -- (0,3);
    \draw[dashed] (1,2) -- (1,-0.5) node[below] {\( a \)};
    \draw[thick,-{Circle[open]}] (1,1) -- (2,2);
    \draw[dashed] (2,0.8) -- (2,-0.5) node[below] {\( b \)};
    \draw[thick,{Circle[open]}-{Circle[open]}] (2,1) -- (3,1);
    \draw[dashed] (3,0.8) -- (3,-0.5) node[below] {\( c \)};
    \draw[thick,{Circle[open]}-] (3,2) -- (4,1);
    \draw[dashed] (4,2) -- (4,-0.5) node[below] {\( d \)};
  \end{tikzpicture}
\end{center}
We can extend over \( [0,\infty) \). A function \( f \) is piecewise continuous
over \( [0,\infty) \) if \( f \) is piecewise continuous over \( [0,N] \) for
all \( N > 0 \).
\[ \int_{a}^{d}f(t) = \int_{a}^{b}f(t)+\int_{b}^{c}f(t)+\int_{c}^{d}f(t) \]

\subsubsection*{Exponential Order \( \alpha \)}
A function \( f \) is of exponential order \( \alpha \) if there exists
positive constants \( M \) and \( T \) such that \( |f(t)|\le M\e^{\alpha t} \)
for all \( t > T \). For example:
\begin{align*}
  f(t) &= \e^{2t}\sin(t) \\
  |\e^{2t}\sin(t)| &= \e^{2t}|\sin(2t)| \le
    M\e^{2t} = \e^{2t} \text{ for all } T \\
  |\sin(2t)| &\le 1
\end{align*}
\( f(t) \) is of exponential order \( \alpha = 2 \).

\subsubsection*{Conditions for Existence of the Laplace Transform}
\begin{enumerate}
  \item If \( f(t) \) is piecewise continuous and of exponential order
  \( \alpha \), then the Laplace transform \( \laplace{f(t)} \) exists for
  \( s>a \).
  \item We need to know that
  \[ \laplace{f(t)} = \int_{0}^{\infty}\e^{-st}f(t)\diff{t} \]
  converges for \( s>a \). We can rewrite it as
  \[ \int_{0}^{\infty}\e^{-st}f(t)\diff{t} = \int_{0}^{T}\e^{-st}f(t)\diff{t}+
    \int_{T}^{\infty}\e^{-st}f(t)\diff{t} \]
  where we have \( |f(t)|\le M\e^{\alpha t} \) for all \( t > T \). By
  continuity, \( \int_{0}^{T}\e^{-st}f(t)\diff{t} \) exists, so we only need to
  consider \( \int_{T}^{\infty}\e^{-st}f(t)\diff{t} \).
  \begin{align*}
    \int_{T}^{\infty}\e^{-st}f(t)\diff{t} &=
      \lim_{N\to\infty}\int_{T}^{N}\e^{-st}f(t)\diff{t} \\
    &\le \lim_{N\to\infty}\int_{T}^{N}M\e^{-st}\e^{\alpha t}\diff{t} \\
    &= \lim_{N\to\infty}M\int_{T}^{N}\e^{-(s-\alpha)t}\diff{t} \\
    &= \lim_{N\to\infty}M\bigg[
      -\frac{1}{s-\alpha}\e^{-(s-\alpha)t}\bigg]_{T}^{N} \\
    &= \lim_{N\to\infty}M\bigg[-\frac{1}{s-\alpha}\e^{-(s-\alpha)N}-
      (-\frac{1}{s-\alpha}\e^{-(s-\alpha)T})\bigg] \\
    &= \frac{M}{s-\alpha}\e^{-(s-\alpha)T} < \infty
  \end{align*}
\end{enumerate}
Since \( M \) and \( T \) are positive constants, this integral converges by
the comparison test for improper integrals.

\subsection*{Properties of the Transform}
\begin{itemize}
  \item Translation in \( s \): If the Laplace transform \( \laplace{f(t)} =
  F(s) \) exists, then \( \laplace{\e^{\alpha t}f(t)} = F(s-a) \).
  \( \e^{\alpha t} \) indicates a translation in the \( s \) domain, where we
  replace \( s \) by \( s-a \) in the transform of \( f(t) \). For example:
  \begin{align*}
    \laplace{\e^{2t}\sin(2t)} & \quad \alpha = 2 \\
    \laplace{\sin(2t)} &= \frac{2}{s^2+4} \\
    \laplace{\e^{2t}\sin(2t)} &= \frac{2}{(s-2)^2+4}
  \end{align*}
  Another example:
  \begin{align*}
    \laplace{\e^{-2t}\cos(2t)} & \quad \alpha = -2 \\
    \laplace{\cos(2t)} &= \frac{s}{s^2+4} \\
    \laplace{\e^{-2t}\cos(2t)} &= \frac{s+2}{(s+2)^2+4}
  \end{align*}
\end{itemize}

\subsection*{The Laplace Transform of the Derivative}
Let \( f \) be continuous on \( [0,\infty) \) and \( f' \) be piecewise
continuous on \( [0,\infty) \) and both are of exponential order \( \alpha \).
\begin{align*}
  \laplace{f'(t)} &= \int_{0}^{\infty}\e^{-st}f'(t)\diff{t} \\
  &= \lim_{N\to\infty}\int_{0}^{N}\e^{-st}f'(t)\diff{t} \\
  u &= \e^{-st} \quad\quad\quad\quad \diff{v} = f'(t)\diff{t} \\
  \diff{u} &= -s\e^{-st}\diff{t} \quad\quad v = f(t) \\
  &= \lim_{N\to\infty}\bigg[\e^{-st}f(t)\bigg]_{0}^{N}+
    \lim_{N\to\infty}s\int_{0}^{N}\e^{-st}f(t)\diff{t} \\
  &= -f(0)+sF(s) \\
  &= sF(s)-f(0)
\end{align*}
In summary:
\begin{align*}
  \laplace{y'} &= sY(s)-y(0) \\
  \laplace{y''} &= s^2Y(s)-sy(0)-y'(0)
\end{align*}

\subsection*{Derivatives of the Laplace Transform}
Let \( F(S) = \laplace{f(t)} \). Then for \( s>a \):
\[ \laplace{t^nf(t)} = (-1)^n\ddiff{^nF}{s^n} \]
For example:
\begin{align*}
  \laplace{t\sin(t)} & \quad n = 1 \quad f(t) = \sin(t) \\
  \laplace{\sin(t)} &= \frac{1}{s^2+1} = F(s) \\
  \ddiff{F}{s} &= \ddiff{}{s}\bigg[\frac{1}{s^2+1}\bigg] \\
  &= \frac{(s^2+1)(0)-1(2s)}{(s^2+1)^2} \\
  &= \frac{-2s}{(s^2+1)^2} \\
  \laplace{t\sin(t)} &= (-1)^1\frac{-2s}{(s^2+1)^2} = \frac{2s}{(s^2+1)^2}
\end{align*}
Another example:
\begin{align*}
  \laplace{t\e^{-2t}\sin(3t)} & \quad n = 1 \quad f(t) = \e^{-2t}\sin(3t) \\
  F(s) &= \laplace{\e^{-2t}\sin(3t)} \\
  \laplace{\sin(3t)} &= \frac{3}{s^2+9} \\
  \laplace{\e^{-2t}\sin(3t)} &= \frac{3}{(s+2)^2+9} = F(s) \\
  \ddiff{}{s}F(s) &= \frac{0-(3(2(s+2)))}{((s+2)^2+9)^2} \\
  &= \frac{-6(s+2)}{((s+2)^2+9)^2} \\
  \laplace{t\e^{-2t}\sin(3t)} &= (-1)^1\frac{-6(s+2)}{((s+2)^2+9)^2} \\
  &= \frac{6(s+2)}{((s+2)^2+9)^2} \\
\end{align*}

\subsection*{Inverse Laplace Transforms}
The Laplace transform maps a function \( f(t) \) to a function \( F(s) =
\laplace{f(t)} \). The transform has an inverse denoted by:
\[ \ilaplace{f(t)} = f(t) \]
Consider the following initial value problem:
\[ y''-y = -t \quad y(0) = 0 \quad y'(0) = 1 \]
If we apply the Laplace transform to the entire equation:
\begin{align*}
  \laplace{y''-y} &= \laplace{-t} \\
  \laplace{y''}-\laplace{y} &= -\laplace{t} \\
  s^2Y(s)-(s)y(0)-y'(0)-Y(s) &= -\frac{1}{s^2} \\
  (s^2-1)Y(s) &= -\frac{1}{s^2}+1 \\
  &= \frac{-1+s^2}{s^2} \\
  Y(s) &= \frac{1}{s^2} \\
  \ilaplace{Y(s)} &= \ilaplace{\frac{1}{s^2}} \\
  t &= y(t)
\end{align*}
Given \( F(s) \), if there exists a function \( f(t) \) that is continuous on
\( [0,\infty) \) where \( \laplace{f(t)} = F(s) \), \( f(t) \) is the inverse
of \( F(s) \). The inverse Laplace transform is a linear operator. Given
\( F_1(s), F_2(s) \) and \( k \) a constant, the properties of linearity apply:
\begin{enumerate}
  \item \( \ilaplace{F_1(s)\pm F_2(s)} =
  \ilaplace{F_1(s)}\pm\ilaplace{F_2(s)} \)
  \item \( \ilaplace{kF_1(s)}\pm = k\ilaplace{F_1} \)
\end{enumerate}

\subsubsection*{Example}
\begin{align*}
  \ilaplace{\frac{3}{s^2+9}} &= \ilaplace{\frac{3}{s^2+3^2}} \\
  &= \sin(3t) \\
  \ilaplace{\frac{s-2}{(s-2)^2+4}} &= \e^{2t}\cos(2t) \\
  \ilaplace{\frac{1}{s-6}} &= \e^{6t}
\end{align*}

\subsubsection*{Review of Partial Fraction Decomposition: Case 1}
Suppose we have \( f(x) = \frac{P(x)}{Q(x)} \) and the degree
of \( P \) is less than the degree of \( Q \).
\[ \frac{P(x)}{Q(x)} =
  \frac{P}{(a_1x+b_1)(a_2x+b_2)\cdot\cdot\cdot(a_nx+b_n)} \]
We have \( n \) distinct linear factors that are irreducible, which we can
rewrite as:
\[ \frac{P(x)}{Q(x)} =
  \frac{A_1}{a_1x+b_1}+\frac{A_2}{a_2x+b_2}+\dots+\frac{A_n}{a_nx+b_n} \]
where all \( A_i \)'s are constants. For example:
\begin{align*}
  \frac{x+4}{x^2+3x+2} &= \frac{x+4}{(x+1)(x+2)} \\
  &= \frac{A}{x+1}+\frac{B}{x+2} = \frac{A(x+2)+B(x+1)}{(x+1)(x+2)} \\
  x+4 &= A(x+2)+B(x+1) \\
  Let: x &= -2 \\
  -2+4 &= -B \quad B = -2 \\
  Let: x &= -1 \\
  A &= 3 \\
\end{align*}
This can be applied to inverse Laplace transforms:
\[ \ilaplace{\frac{3s+2}{s^2+s-2}} \]
\begin{align*}
  \frac{3s+2}{s^2+s-2} &= \frac{3s+2}{(s+2)(s-1)} \\
  &= \frac{A}{s+2}+\frac{B}{s-1} \\
  &= \frac{A(s-1)+B(s+2)}{(s+2)(s-1)} \\
  3s+2 &= A(s-1)+B(s+2) \\
  Let: s &= 1 \quad 5 = 3B \quad B = \frac{5}{3} \\
  Let: s &= -2 \quad A = \frac{4}{3}
\end{align*}
\begin{align*}
  \ilaplace{\frac{3s+2}{s^2+s-2}} &=
    \ilaplace{\frac{4}{3}\frac{1}{s-1}+\ilaplace{\frac{5}{3}\frac{1}{s+2}}} \\
  &= \frac{4}{3}\ilaplace{\frac{1}{s-1}}+\frac{5}{3}\ilaplace{\frac{1}{s+2}} \\
  &= \frac{4}{3}\e^t+\frac{5}{3}\e^{-2t}
\end{align*}

\subsubsection*{Review of Partial Fraction Decomposition: Case 2}
In this case, we can have \( n \) repeated linear factors:
\[ f(x) = \frac{P(x)}{Q(x)} = \frac{P(x)}{(a_1x+b_1)^n} = \frac{A_1}{a_1x+b_1}+
  \frac{A_2}{(a_1x+b_1)^2}+\dots+\frac{A_n}{(a_1x+b_1)^n} \]
For example:
\[ \ilaplace{\frac{s^2+9s+2}{(s-2)^2(s+3)}} \]
\begin{align*}
  \frac{A}{s+3}+\frac{B}{s-1}+\frac{C}{(s-1)^2}
    &= \frac{A(s-1)^2+B(s+3)(s-1)+C(s+3)}{(s-1)^2(s+3)} \\
  s^2+9s+2 &= A(s-1)^2+B(s+3)(s-1)+C(s+3) \\
  Let: s &= 1 \\
  1+9+2 &= 4C \quad 4C = 12 \quad C = 3 \\
  Let: s &= -3 \\
  9-27+2 &= 16A \quad A = -1 \\
  Let: S &= 0 \\
  2 &= -1-3B+3C \quad B = 2 \\
  \ilaplace{\frac{s^2+9s+2}{(s-2)^2(s+3)}} &= \ilaplace{\frac{-1}{s+3}+
    \frac{2}{s-1}+\frac{3}{(s-1)^2}} \\
  &= -\ilaplace{\frac{1}{s+3}}+2\ilaplace{\frac{1}{s-1}}+
    3\ilaplace{\frac{1}{(s-1)^2}} \\
  &= -\e^{-3t}+2\e^t+3t\e^t
\end{align*}

\subsubsection*{Review of Partial Fraction Decomposition: Case 3}
In this case, we have \( n \) irreducible distinct quadratics:
\begin{align*}
  \frac{P(x)}{Q(x)} &=
    \frac{P(x)}{(a_1x^2+b_1x+c)\cdot\cdot\cdot(a_nx^2+b_nx+c_n)} \\
  &= \frac{A_1x+B_1}{a_1x^2+b_1x+c_1}+\dots+\frac{A_nx+B_n}{a_nx^2+b_nx+c_n} \\
\end{align*}
For example:
\[ \ilaplace{\frac{7s-8}{(s^2+4)(s+1)(s-2)}} \]
\begin{align*}
  \frac{7s-8}{(s^2+4)(s+1)(s-2)} &=
    \frac{A}{s-1}+\frac{B}{s-2}+\frac{Cs+D}{s^2+4} \\
  7s-8 &= A(s-2)(s^2+4)+B(s+1)(s^2+4)+(Cs+D)(s+1)(s-2) \\
  Let: s &= 2 \quad B = \frac{1}{4} \\
  Let: s &= -1 \quad A = 1 \\
  Let: s &= 0 \quad D = \frac{1}{2} \\
  Let: s &= 1 \quad C = -\frac{5}{4} \\
  \ilaplace{\frac{7s-8}{(s^2+4)(s+1)(s-2)}} &= \ilaplace{\frac{1}{s+1}}+
    \ilaplace{\frac{1}{4}\frac{1}{s-2}}+
    \ilaplace{\frac{-\frac{5}{4}s+\frac{1}{2}}{s^2+4}} \\
  &= \ilaplace{\frac{1}{s+1}}+\frac{1}{4}\ilaplace{\frac{1}{s-2}}-
    \frac{5}{4}\ilaplace{\frac{s}{s^2+4}}+
    \frac{1}{2}\ilaplace{\frac{1}{s^2+4}} \\
  &= \e^{-t}+\frac{1}{4}\e^{2t}-\frac{5}{4}\cos(2t)+\frac{1}{4}\sin(2t)
\end{align*}


\begin{center}
  You can find all my notes at \url{http://omgimanerd.tech/notes}. If you have
  any questions, comments, or concerns, please contact me at
  alvin@omgimanerd.tech
\end{center}

\end{document}
