\documentclass{math}

\usepackage{graphicx}

\geometry{letterpaper, margin=0.5in}

\title{Differential Equations: Homework 11}
\author{Alvin Lin}
\date{January 2018 - May 2018}

\begin{document}

\maketitle
\clearpage

\section*{Section 7.5}

\subsubsection*{Exercise 2}
Solve the given initial value problem using the method of Laplace transforms.
\begin{align*}
  y''-y'-2y &= 0 \quad y(0) = -2 \quad y'(0) = 5 \\
  \laplace{y''-y'-2y} &= \laplace{0} \\
  \laplace{y''}-\laplace{y'}-2\laplace{y} &= 0 \\
  \bigg[s^2Y(s)-sy(0)-y'(0)\bigg]-\bigg[sY(s)-y(0)\bigg]-2(Y(s)) &= 0 \\
  s^2Y(s)+2s-5-sY(s)-2-2Y(s) &= 0 \\
  s^2Y(s)-sY(s)-2Y(s) &= 7-2s \\
  Y(s)(s^2-s-2) &= 7-2s \\
  Y(s) &= \frac{7-2s}{s^2-s-2} \\
  y(t) &= \ilaplace{Y(s)} \\
  \frac{A}{s-2}+\frac{B}{s+1} &= \frac{7-2s}{(s-2)(s+1)} \\
  A(s+1)+B(s-2) &= 7-2s \\
  Let: s = -1 \quad B &= -3 \\
  Let: s = 2 \quad A &= 1 \\
  y(t) &= \ilaplace{\frac{1}{s-2}-\frac{3}{s+1}} \\
  &= \ilaplace{\frac{1}{s-2}}-3\ilaplace{\frac{1}{s+1}} \\
  &= \e^{2t}-3\e^{-t}
\end{align*}

\subsubsection*{Exercise 3}
Solve the given initial value problem using the method of Laplace transforms.
\begin{align*}
  y''+6y'+9y &= 0 \quad y(0) = -1 \quad y'(0) = 6 \\
  \laplace{y''+6y'+9y} &= \laplace{0} \\
  \laplace{y''}+6\laplace{y'}+9\laplace{y} &= 0 \\
  \bigg[s^2Y(s)-sy(0)-y'(0)\bigg]+6\bigg[sY(s)-y(0)\bigg]+9(Y(s)) &= 0 \\
  s^2Y(s)+s-6+6sY(s)+6+9Y(s) &= 0 \\
  s^2Y(s)+6sY(s)+9Y(s) &= -s \\
  Y(s)(s^2+6s+9) &= -s \\
  Y(s) &= \frac{-s}{s^2+6s+9} \\
  y(t) &= \ilaplace{Y(s)} \\
  \frac{A}{(s+3)^2}+\frac{B}{s+3} &= \frac{-s}{(s+3)^2} \\
  A+B(s+3) &= -s \\
  Let: s = -3 \quad A &= 3 \\
  Let: s = 1 \quad B &= -1 \\
  y(t) &= \ilaplace{\frac{3}{(s+3)^2}-\frac{1}{s+3}} \\
  &= 3\ilaplace{\frac{1}{(s+3)^2}}-\ilaplace{\frac{1}{s+3}} \\
  &= 3t\e^{3t}-\e^{3t}
\end{align*}

\subsubsection*{Exercise 4}
Solve the given initial value problem using the method of Laplace transforms.
\begin{align*}
  y''+6y'+5y &= 12\e^t \quad y(0) = -1 \quad y'(0) = 7 \\
  \laplace{y''+6y'+5y} &= \laplace{12\e^t} \\
  \laplace{y''}+6\laplace{y'}+5\laplace{y} &= 12\laplace{\e^t} \\
  \bigg[s^2Y(s)-sy(0)-y'(0)\bigg]+6\bigg[sY(s)-y(0)\bigg]+5Y(s) &=
    12\frac{1}{s-1} \\
  s^2Y(s)+s-7+6sY(s)+6+5Y(s) &= \frac{12}{s-1} \\
  s^2Y(s)+6sY(s)+5Y(s) &= \frac{12}{s-1}-s+1 \\
  Y(s)(s^2+6s+5) &= \frac{12}{s-1}-s+1 \\
  Y(s) &= \frac{12}{(s-1)(s+5)(s+1)}-\frac{s-1}{(s+5)(s+1)} \\
  y(t) &= \ilaplace{Y(s)} \\
  \frac{A}{s-1}+\frac{B}{s+5}+\frac{C}{s+1} &= \frac{12}{(s-1)(s+5)(s+1)}
\end{align*}
\[ A(s+5)(s+1)+B(s-1)(s+1)+C(s-1)(s+5) = 12 \]
\begin{align*}
  Let: s = -5 \quad B &= \frac{1}{2} \\
  Let: s = -1 \quad C &= -\frac{3}{2} \\
  Let: s = 1 \quad A &= 1 \\
  \frac{D}{s+5}+\frac{E}{s+1} &= \frac{s-1}{(s+5)(s+1)} \\
  D(s+1)+E(s+5) &= s-1 \\
  Let: s = -5 \quad D &= \frac{3}{2} \\
  Let: s = -1 \quad E &= -\frac{1}{2} \\
  Y(s) &= \frac{1}{s-1}+\frac{1}{2}\frac{1}{s+5}-\frac{3}{2}\frac{1}{s+1}
    -\frac{3}{2}\frac{1}{s+5}+\frac{1}{2}\frac{1}{s+1} \\
  y(t) &= \ilaplace{\frac{1}{s-1}-\frac{1}{s+5}-\frac{1}{s+1}} \\
  &= \ilaplace{\frac{1}{s-1}}-\ilaplace{\frac{1}{s+5}}-
    \ilaplace{\frac{1}{s+1}} \\
  &= \e^{t}-\e^{-5t}-\e^{-t}
\end{align*}

\subsubsection*{Exercise 7}
Solve the given initial value problem using the method of Laplace transforms.
\begin{align*}
  y''-7y'+10y &= 9\cos(t)+7\sin(t) \quad y(0) = 5 \quad y'(0) = -4 \\
  \laplace{y''-7y'+10y} &= \laplace{9\cos(t)+7\sin(t)} \\
  \laplace{y''}-7\laplace{y'}+10\laplace{y} &=
    9\laplace{\cos(t)}+7\laplace{\sin(t)} \\
  \bigg[s^2Y(s)-sy(0)-y'(0)\bigg]-7\bigg[sY(s)-y(0)\bigg]+10Y(s) &=
    9\frac{s}{s^2+1}+7\frac{1}{s^2+1} \\
  s^2Y(s)-5s+4-7sY(s)+35+10Y(s) &= \frac{9s+7}{s^2+1} \\
  s^2Y(s)-7sY(s)+10Y(s) &= \frac{9s+7}{s^2+1}+5s-39 \\
  Y(s) &= \frac{9s+7}{(s^2+1)(s-2)(s-5)}+\frac{5s-39}{(s-2)(s-5)} \\
  &= \frac{5s^3-39s^2+14s-32}{(s^2+1)(s-2)(s-5)} \\
  \frac{As+B}{s^2+1}+\frac{C}{s-2}+\frac{D}{s-5} &=
    \frac{5s^3-39s^2+14s-32}{(s^2+1)(s-2)(s-5)}
\end{align*}
\[ (As+B)(s-2)(s-5)+C(s^2+1)(s-5)+D(s^2+1)(s-2) = 5s^3-39s^2+14s-32 \]
\begin{align*}
  Let: s = 2 \quad C &= 8 \\
  Let: s = 5 \quad D &= -4 \\
  Let: s = 0 \quad B &= 0 \\
  Let: s = 1 \quad A &= 1 \\
  Y(s) &= \frac{s}{s^2+1}+\frac{8}{s-2}-\frac{4}{s-5} \\
  y(t) &= \ilaplace{\frac{s}{s^2+1}}+8\ilaplace{\frac{1}{s-2}}-
    4\ilaplace{\frac{1}{s-5}} \\
  &= \cos(t)+8\e^{2t}-4\e^{5t}
\end{align*}

\subsubsection*{Exercise 10}
Solve the given initial value problem using the method of Laplace transforms.
\begin{align*}
  y''-4y &= 4t-8\e^{-2t} \quad y(0) = 0 \quad y'(0) = 5 \\
  \laplace{y''-4y} &= \laplace{4t-8\e^{-t}} \\
  \laplace{y''}-4\laplace{y} &= 4\laplace{t}-8\laplace{\e^{-t}} \\
  \bigg[s^2Y(s)-sy(0)-y'(0)\bigg]-4Y(s) &= 4\frac{1}{s^2}-8\frac{1}{s+1} \\
  s^2Y(s)-5-4Y(s) &= \frac{4}{s^2}-\frac{8}{s+1} \\
  Y(s)(s^2-4) &= \frac{4}{s^2}-\frac{8}{s+2}+5 \\
  Y(s) &= \frac{4}{s^2(s^2-4)}-\frac{8}{(s+2)(s^2-4)}+\frac{5}{s^2-4} \\
  &= \frac{5s^3+2s^2+4s+8}{s^2(s^2-4)(s+2)} \\
  &= \frac{5s^3+2s^2+4s+8}{s^2(s+2)(s-2)(s+2)} \\
  \frac{A}{s}+\frac{B}{s^2}+\frac{C}{s+2}+\frac{D}{(s+2)^2}+\frac{E}{s-2} &=
    \frac{5s^3+2s^2+4s+8}{s^2(s+2)(s-2)(s+2)} \\
\end{align*}
\[ As(s+2)^2(s-2)+B(s+2)^2(s-2)+Cs^2(s+2)(s-2)+Ds^2(s-2)+Es^2(s+2)^2 =
  5s^3+2s^2+4s+8\]
\begin{align*}
  Let: s = -2 \quad D &= 2 \\
  Let: s = 2 \quad E &= 1 \\
  Let: s = 0 \quad B &= -1 \\
  A &= 0 \quad \text{via system of equations}\\
  C &= -1 \\
  Y(s) &= -\frac{1}{s^2}-\frac{1}{s+2}+\frac{2}{(s+2)^2}+\frac{1}{s-2} \\
  y(t) &= -\ilaplace{\frac{1}{s^2}}-\ilaplace{\frac{1}{s+2}}+
    2\ilaplace{\frac{1}{(s+2)^2}}+ \ilaplace{\frac{1}{s-2}} \\
  &= -t-\e^{-2t}+2t\e^{-2t}+\e^{2t}
\end{align*}

\begin{center}
  If you have any questions, comments, or concerns, please contact me at
  alvin@omgimanerd.tech
\end{center}

\end{document}
