\documentclass{math}

\usepackage{tikz}
\usetikzlibrary{arrows.meta}

\geometry{letterpaper, margin=0.5in}

\title{Differential Equations: Homework 12}
\author{Alvin Lin}
\date{January 2018 - May 2018}

\begin{document}

\maketitle
\clearpage

\section*{Section 7.6}

\subsubsection*{Exercise 2}
Sketch the graph of the given function and determine its Laplace transform.
\[ u(t-1)-u(t-4) \]
\begin{center}
  \begin{tikzpicture}[shorten >=-2.5pt,shorten <=-2.5pt]
    \draw[<->] (0,-2) -- (0,2);
    \draw[->] (0,0) -- (5,0);
    \draw[thick,-{Circle[open]}] (0,0) -- (1,0);
    \draw[thick,{Circle[open]}-{Circle[open]}] (1,1) -- (4,1);
    \draw[thick,{Circle[open]}-] (4,0) -- (5,0);
  \end{tikzpicture}
\end{center}
\begin{align*}
  \laplace{u(t-1)-u(t-4)} &= \laplace{u(t-1)}-\laplace{u(t-4)} \\
  &= \frac{\e^{-s}}{s}-\frac{\e^{-4s}}{s}
\end{align*}

\subsubsection*{Exercise 5}
Express the given function using window and step functions and compute its
Laplace transform.
\begin{align*}
  g(t) &= \begin{cases}
    0, &\quad 0<t<1 \\
    2, &\quad 1<t<2 \\
    1, &\quad 2<t<3 \\
    3, &\quad 3<t
  \end{cases}
\end{align*}
\begin{center}
  \begin{tikzpicture}[shorten >=-2.5pt,shorten <=-2.5pt]
    \draw[<->] (0,-2) -- (0,2);
    \draw[->] (0,0) -- (5,0);
    \draw[thick,-{Circle[open]}] (0,0) -- (1,0);
    \draw[thick,{Circle[open]}-{Circle[open]}] (1,2) -- (2,2);
    \draw[thick,{Circle[open]}-{Circle[open]}] (2,1) -- (3,1);
    \draw[thick,{Circle[open]}-] (3,3) -- (5,3);
  \end{tikzpicture}
\end{center}
\begin{align*}
  g(t) &= 0+2u(t-1)-u(t-2)+2u(t-3) \\
  \laplace{g(t)} &= 2\laplace{u(t-1)}-\laplace{u(t-2)}+2\laplace{u(t-3)} \\
  &= \frac{2\e^{-s}}{s}-\frac{\e^{-2s}}{s}+\frac{2\e^{-3s}}{s}
\end{align*}

\subsubsection*{Exercise 6}
Express the given function using window and step functions and compute its
Laplace transform.
\begin{align*}
  g(t) &= \begin{cases}
    0, &\quad 0<t<2 \\
    t+1, &\quad 2<t
  \end{cases} \\
  &= (t+1)u(t-2) \\
  \laplace{g(t)} &= \laplace{(t+1)u(t-2)} \\
  &= \e^{-2s}\laplace{(t+1)+2} \\
  &= \e^{-2s}\laplace{t+3} \\
  &= \e^{-2s}(\laplace{t}+3\laplace{1}) \\
  &= \e^{-2s}(\frac{1}{s^2}+\frac{3}{s})
\end{align*}

\subsubsection*{Exercise 11}
Determine an inverse Laplace transform of the given function.
\begin{align*}
  \ilaplace{\frac{\e^{-2s}}{s-1}} &= \ilaplace{\e^{-as}F(s)} \\
  &= f(t-a)u(t-a) \\
  a &= 2 \\
  F(s) &= \frac{1}{s-1} \\
  f(t) &= \e^t \\
  f(t-a)u(t-a) &= \e^{t-2}u(t-2)
\end{align*}

\subsubsection*{Exercise 12}
Determine an inverse Laplace transform of the given function.
\begin{align*}
  \ilaplace{\frac{\e^{-3s}}{s^2}} &= \ilaplace{\e^{-as}F(s)} \\
  &= f(t-a)u(t-a) \\
  a &= 3 \\
  F(s) &= \frac{1}{s^2} \\
  f(t) &= t \\
  f(t-a)u(t-a) &= (t-3)u(t-3)
\end{align*}

\subsubsection*{Exercise 13}
Determine an inverse Laplace transform of the given function.
\begin{align*}
  \ilaplace{\frac{\e^{-2s}-3\e^{-4s}}{s+2}} &=
    \ilaplace{\frac{\e^{-2s}}{s+2}}-3\ilaplace{\frac{\e^{-4s}}{s+2}} \\
  a_1 &= 2 \\
  F(s) &= \frac{1}{s+2} \\
  f(t) &= \e^{-2t} \\
  \ilaplace{\frac{\e^{-2s}}{s+2}} &= f(t-a_1)u(t-a_1) \\
  &= \e^{-2(t-2)}u(t-2) \\
  a_2 &= 4 \\
  \ilaplace{\frac{\e^{-4s}}{s+2}} &= f(t-a_2)u(t-a_2) \\
  &= \e^{-2(t-4)}u(t-4) \\
  \ilaplace{\frac{\e^{-2s}}{s+2}}-3\ilaplace{\frac{\e^{-4s}}{s+2}} &=
    \e^{-2t+4}u(t-2)-3\e^{-2t+8}u(t-4)
\end{align*}

\subsubsection*{Exercise 14}
Determine an inverse Laplace transform of the given function.
\begin{align*}
  \ilaplace{\frac{\e^{-3s}}{s^2+9}} &= \ilaplace{\e^{-as}F(s)} \\
  &= f(t-a)u(t-a) \\
  a &= 3 \\
  F(s) &= \frac{1}{s^2+9} \\
  &= \frac{1}{3}\frac{3}{s^2+9} \\
  f(t) &= \frac{1}{3}\sin(3t) \\
  f(t-a)u(t-a) &= \frac{1}{3}\sin(3(t-3))u(t-3) \\
  &= \frac{1}{3}\sin(3t-9)u(t-3)
\end{align*}

\subsubsection*{Exercise 17}
Determine an inverse Laplace transform of the given function.
\begin{align*}
  \ilaplace{\frac{\e^{-3s}(s-5)}{(s+1)(s+2)}} &= \ilaplace{\e^{-as}F(s)} \\
  &= f(t-a)u(t-a) \\
  a &= 3 \\
  F(s) &= \frac{s-5}{(s+1)(s+2)} \\
  \frac{A}{s+1}+\frac{B}{s+2} &= \frac{s-5}{(s+1)(s+2)} \\
  A(s+2)+B(s+1) &= s-5 \\
  Let: s = -2 \quad B &= 7 \\
  Let: s = -1 \quad A &= -6 \\
  F(s) &= \frac{-6}{s+1}+\frac{7}{s+2} \\
  f(t) &= \ilaplace{F(s)} \\
  &= -6\ilaplace{\frac{1}{s+1}}+7\ilaplace{\frac{1}{s+2}} \\
  &= -6\e^{-t}+7\e^{-2t} \\
  f(t-a)u(t-a) &= (-6\e^{-(t-3)}+7\e^{-2(t-3)})u(t-3) \\
  &= (-6\e^{-t+3}+7\e^{-2t+6})u(t-3)
\end{align*}

\subsubsection*{Exercise 21}
Solve the given initial value problem using the method of Laplace transforms.
Sketch the graph of the solution.
\begin{align*}
  y''+y &= u(t-3) \quad y(0) = 0 \quad y'(0) = 1 \\
  \laplace{y''+y} &= \laplace{u(t-3)} \\
  s^2Y(s)-sy(0)-y'(0)+Y(s) &= \frac{\e^{-3s}}{s} \\
  s^2Y(s)-1+Y(s) &= \frac{\e^{-3s}}{s} \\
  Y(s)(s^2+1)-1 &= \frac{\e^{-3s}}{s} \\
  Y(s)(s^2+1) &= \frac{\e^{-3s}}{s}+1 \\
  Y(s) &= \frac{\e^{-3s}}{s(s^2+1)}+\frac{1}{s^2+1} \\
  y(t) &= \ilaplace{Y(s)} \\
  &= \ilaplace{\frac{\e^{-3s}}{s(s^2+1)}}+\ilaplace{\frac{1}{s^2+1}}
\end{align*}
\begin{align*}
  \ilaplace{\frac{\e^{-3s}}{s(s^2+1)}} &= \ilaplace{\e^{-as}F(s)} \\
  a &= 3 \\
  F(s) &= \frac{1}{s(s^2+1)} \\
  &= \frac{A}{s}+\frac{Bs+C}{s^2+1} \\
  A(s^2+1)+(Bs+C)s &= 1 \\
  (A+B)s^2+Cs+A &= 1 \\
  A = 1 \quad A+B &= 0 \quad C = 0 \quad B = -1 \\
  F(s) &= \frac{1}{s}-\frac{s}{s^2+1} \\
  f(t) &= 1-\cos(t) \\
  f(t-a)u(t-a) &= (1-\cos(t-3))u(t-3) \\
  y(t) &= (1-\cos(t-3))u(t-3)+\sin(t) \\
  &= u(t-3)-\cos(t-3)u(t-3)+\sin(t)
\end{align*}

\subsubsection*{Exercise 29}
Solve the given initial value problem using the method of Laplace transforms.
Sketch the graph of the solution.
\begin{align*}
  y''+4y &= g(t) \quad y(0) = 1 \quad y'(0) = 3 \\
  g(t) &= \begin{cases}
    \sin(t), &\quad 0\le t\le 2\pi \\
    0, &\quad 2\pi<t
  \end{cases} \\
  &= \sin(t)-\sin(t)u(t-2\pi) \\
  \laplace{y''+4y} &= \laplace{g(t)} \\
  s^2Y(s)-sy(0)-y'(0)+4Y(s) &= \frac{1}{s^2+1}-\frac{\e^{-2\pi s}}{s^2+1} \\
  s^2Y(s)-s-3+4Y(s) &= \frac{1}{s^2+1}-\frac{\e^{-2\pi s}}{s^2+1} \\
  Y(s)(s^2+4) &= \frac{1}{s^2+1}-\frac{\e^{-2\pi s}}{s^2+1}+s+3 \\
  Y(s) &= \frac{1}{(s^2+1)(s^2+4)}-\frac{\e^{-2\pi s}}{(s^2+1)(s^2+4)}+
    \frac{s+3}{s^2+4} \\
  & \text{partial fraction decomposition omitted for brevity} \\
  y(t) &= \ilaplace{Y(s)} \\
  \ilaplace{\frac{1}{(s^2+1)(s^2+4)}} &=
    \ilaplace{\frac{1}{3}\frac{1}{s^2+1}-\frac{1}{3}\frac{1}{s^2+4}} \\
  &= \frac{1}{3}\ilaplace{\frac{1}{s^2+1}}-
    \frac{1}{6}\ilaplace{\frac{2}{s^2+4}} \\
  &= \frac{1}{3}\sin(t)-\frac{1}{6}\sin(2t)
\end{align*}
\begin{align*}
  \ilaplace{\frac{\e^{-2\pi s}}{(s^2+1)(s^2+4)}} &= \ilaplace{\e^{-as}F(s)} \\
  a &= 2\pi \\
  F(s) &= \frac{1}{(s^2+1)(s^2+4)} \\
  f(t) &= \frac{1}{3}\sin(t)-\frac{1}{6}\sin(2t) \\
  f(t-a)u(t-a) &= (\frac{1}{3}\sin(t-2\pi)-\frac{1}{6}\sin(2t-4\pi))u(t-2\pi) \\
  &= \frac{u(t-2\pi)}{3}\sin(t)-\frac{u(t-2\pi)}{6}\sin(2t) \\
  \ilaplace{\frac{s+3}{s^2+4}} &=
    \ilaplace{\frac{s}{s^2+4}}+\ilaplace{\frac{3}{s^2+4}} \\
  &= \ilaplace{\frac{s}{s^2+4}}+\frac{3}{2}\ilaplace{\frac{2}{s^2+4}} \\
  &= \cos(2t)+\frac{3}{2}\sin(2t) \\
  y(t) &= \frac{1}{3}\sin(t)-\frac{1}{6}\sin(2t)+
    \frac{u(t-2\pi)}{3}\sin(t)-\frac{u(t-2\pi)}{6}\sin(2t)+
    \cos(2t)+\frac{3}{2}\sin(2t) \\
  &= \frac{1-u(t-2\pi)}{3}\sin(t)-\frac{8+u(t-2\pi)}{6}\sin(2t)+\cos(2t) \\
\end{align*}

\section*{Section 7.9}

\subsubsection*{Exercise 5}
Evaluate the given integral:
\begin{align*}
  \int_{0}^{\infty}\e^{-2t}\delta(t-1)\diff{t} &=
    \int_{0}^{\infty}f(t)\delta(t-1)\diff{t} \\
  f(t) &= \e^{-2t} \\
  \int_{0}^{\infty}\e^{-2t}\delta(t-1)\diff{t} &= f(a) \\
  &= \e^{-2}
\end{align*}

\subsubsection*{Exercise 7}
Determine the Laplace transform of the given generalized function.
\begin{align*}
  \laplace{\delta(t-1)-\delta(t-3)} &=
    \laplace{\delta(t-1)}-\laplace{\delta(t-3)} \\
  &= \e^{-s}-\e^{-3s}
\end{align*}

\subsubsection*{Exercise 8}
Determine the Laplace transform of the given generalized function.
\begin{align*}
  \laplace{3\delta(t-1)} &= 3\laplace{\delta(t-1)} \\
  &= 3\e^{-s}
\end{align*}

\subsubsection*{Exercise 13}
Solve the given symbolic initial value problem.
\begin{align*}
  w''+w &= \delta(t-\pi) \quad w(0) = 0 \quad w'(0) = 0 \\
  \laplace{w''+w} &= \laplace{\delta(t-\pi)} \\
  s^2W(s)-sw(0)-w'(0)+W(s) &= \e^{-\pi s} \\
  W(s)(s^2+1) &= \e^{-\pi s} \\
  W(s) &= \frac{\e^{-\pi s}}{s^2+1} \\
  w(t) &= \ilaplace{\frac{\e^{-\pi s}}{s^2+1}} \\
  &= \ilaplace{\e^{-as}F(s)} \\
  a &= \pi \\
  F(s) &= \frac{1}{s^2+1} \\
  f(t) &= \ilaplace{F(s)} = \sin(t) \\
  w(t) &= f(t-a)u(t-a) = \sin(t-\pi)u(t-\pi)
\end{align*}

\subsubsection*{Exercise 15}
Solve the given symbolic initial value problem.
\begin{align*}
  y''+2y'-3y &= \delta(t-1)-\delta(t-2) \quad y(0) = 2 \quad y'(0) = -2 \\
  \laplace{y''+2y'-3y} &= \laplace{\delta(t-1)-\delta(t-2)} \\
  s^2Y(s)-sy(0)-y'(0)+2(sY(s)-y(0))-3Y(s) &= \e^{-s}-\e^{-2s} \\
  s^2Y(s)-2s+2+2sY(s)-4-3Y(s) &= \e^{-s}-\e^{-2s} \\
  Y(s)(s^2+2s-3)-2s-2 &= \e^{-s}-\e^{-2s} \\
  Y(s) &= \frac{\e^{-s}-\e^{-2s}+2s+2}{s^2+2s-3}
\end{align*}
\[ y(t) = \ilaplace{\frac{\e^{-s}}{(s+3)(s-1)}}-
    \ilaplace{\frac{\e^{-2s}}{(s+3)(s-1)}}+
    2\ilaplace{\frac{s}{(s+3)(s-1)}}+
    2\ilaplace{\frac{1}{(s+3)(s-1)}} \]
\begin{align*}
  \text{partial fraction decomposition omitted for brevity} \\
  \ilaplace{\frac{\e^{-s}}{(s+3)(s-1)}} &=
    \frac{1}{4}\ilaplace{\frac{\e^{-s}}{s-1}}-
    \frac{1}{4}\ilaplace{\frac{\e^{-s}}{s+3}} \\
  &= \frac{\e^{t-1}}{4}u(t-1)-\frac{\e^{3-t}}{4}u(t-1) \\
  &= \frac{\e^{t-1}-\e^{3-t}}{4}u(t-1) \\
  \ilaplace{\frac{\e^{-2s}}{(s+3)(s-1)}} &=
    \frac{1}{4}\ilaplace{\frac{\e^{-2s}}{s-1}}-
    \frac{1}{4}\ilaplace{\frac{\e^{-2s}}{s+3}} \\
  &= \frac{\e^{t-2}}{4}u(t-2)-\frac{\e^{6-3t}}{4}u(t-2) \\
  &= \frac{\e^{t-2}-\e^{6-3t}}{4}u(t-2) \\
\end{align*}
\begin{align*}
  2\ilaplace{\frac{s}{(s+3)(s-1)}} &=
    \frac{1}{2}\ilaplace{\frac{1}{s-1}}+\frac{3}{2}\ilaplace{\frac{1}{s+3}} \\
  &= \frac{\e^{t}}{2}+\frac{3\e^{-3t}}{2} \\
  2\ilaplace{\frac{1}{(s+3)(s-1)}} &=
    \frac{1}{2}\ilaplace{\frac{1}{s-1}}-\frac{1}{2}\ilaplace{\frac{1}{s+3}} \\
  &= \frac{\e^{t}}{2}-\frac{\e^{-3t}}{2} \\
  y(t) &= \frac{\e^{t-1}-\e^{3-t}}{4}u(t-1)-
    \frac{\e^{t-2}-\e^{6-3t}}{4}u(t-2)+
    \frac{\e^{t}}{2}+\frac{3\e^{-3t}}{2}+
    \frac{\e^{t}}{2}-\frac{\e^{-3t}}{2} \\
  &= \frac{\e^{t-1}-\e^{3-t}}{4}u(t-1)-
    \frac{\e^{t-2}-\e^{6-3t}}{4}u(t-2)+\e^t+\e^{-3t}
\end{align*}

\subsubsection*{Exercise 16}
Solve the given symbolic initial value problem.
\begin{align*}
  y''-2y'-3y &= 2\delta(t-1)-\delta(t-3) \quad y(0) = 2 \quad y'(0) = 2 \\
  \laplace{y''-2y'-3y} &= \laplace{2\delta(t-1)-\delta(t-3)} \\
  s^2Y(s)-sy(0)-y'(0)-2(sY(s)-y(0))-3Y(s) &= 2\e^{-s}-\e^{-3s} \\
  s^2Y(s)-2s-2-2sY(s)+4-3Y(s) &= 2\e^{-s}-\e^{-3s} \\
  Y(s)(s^2-2s-3) &= 2\e^{-s}-\e^{-3s}+2s-2 \\
  Y(s) &= \frac{2\e^{-s}-\e^{-3s}+2s-2}{(s-3)(s+1)}
\end{align*}
\begin{align*}
  Y(s) &= 2\frac{\e^{-s}}{(s-3)(s+1)}-
    \frac{\e^{-3s}}{(s-3)(s+1)}+
    2\frac{s}{(s-3)(s+1)}-
    2\frac{1}{(s-3)(s+1)} \\
  & \text{partial fraction decomposition omitted for brevity} \\
  &= \frac{1}{2}\frac{\e^{-s}}{s-3}-\frac{1}{2}\frac{\e^{-s}}{s+1}-
    \frac{1}{4}\frac{\e^{-3s}}{s-3}+\frac{1}{4}\frac{\e^{-3s}}{s+1}+
    \frac{3}{2}\frac{1}{s-3}+\frac{1}{2}\frac{1}{s+1}-
    \frac{1}{2}\frac{1}{s-3}+\frac{1}{2}\frac{1}{s+1} \\
  &= \frac{1}{2}\frac{\e^{-s}}{s-3}-\frac{1}{2}\frac{\e^{-s}}{s+1}-
    \frac{1}{2}\frac{\e^{-3s}}{s-3}+\frac{1}{4}\frac{\e^{-3s}}{s+1}+
    \frac{1}{s-3}+\frac{1}{s+1} \\
  y(t) &= \ilaplace{Y(s)} \\
  &= \frac{\e^{3t-3}}{2}u(t-1)-\frac{\e^{1-t}}{2}u(t-1)-
    \frac{\e^{3t-9}}{4}u(t-3)-\frac{\e^{3-t}}{4}u(t-3)+
    \e^{3t}+\e^{-t} \\
  &= \frac{\e^{3t-3}-\e^{1-t}}{2}u(t-1)-\frac{\e^{3t-9}-\e^{3-t}}{4}u(t-3)+
    \e^{3t}+\e^{-t}
\end{align*}

\begin{center}
  If you have any questions, comments, or concerns, please contact me at
  alvin@omgimanerd.tech
\end{center}

\end{document}
