\documentclass{math}

\usepackage{enumerate}

\geometry{letterpaper, margin=0.5in}

\title{Boundary Value Problems: Homework 2}
\author{Alvin Lin}
\date{August 2018 - December 2018}

\begin{document}

\maketitle

\subsubsection*{Problem 1}
Complete Exercises 1.2 problems 1, 2, 3, 5 \\
\textbf{Problem 1} \\
Determine a general solution for the equation \( y''+5y'+6y = 0 \).
\begin{align*}
  y''+5y'+6y &= 0 \\
  y &= \e^{rt} \\
  r^2+5r+6 &= (r+2)(r+3) = 0 \\
  r_1 &= -2 \quad r_2 = -3 \\
  y &= c_1\e^{-2t}+c_2\e^{-3t}
\end{align*}
\textbf{Problem 2} \\
Find a general solution for the equation \( y''-4y'+4y = 0 \).
\begin{align*}
  y''-4y'+4y &= 0 \\
  r^2-4r+4 &= 0 \\
  r_{1,2} &= -2 \\
  y &= \e^{-2t}+t\e^{-2t}
\end{align*}
\textbf{Problem 3} \\
Solve the differential equation \( y''+2y'+2y = 0 \).
\begin{align*}
  y''+2y'+2y &= 0 \\
  r^2+2r+2 &= 0 \\
  r &= \frac{-2+\sqrt{4-(4)(1)(2)}}{2} \\
  &= -1\pm i \quad \alpha = -1 \quad \beta = 1 \\
  y &= \e^{-t}\left[c_1\cos(t)+c_2\sin(t)\right]
\end{align*}
\textbf{Problem 5} \\
Solve the boundary value problem \( y''-y = 0, y(0) = 0, y'(\pi) = 1 \).
\begin{align*}
  y''-y &= 0 \\
  r^2-1 &= (r+1)(r-1) = 0 \\
  r_1 &= -1 \quad r_2 = 1 \\
  y &= c_1\e^{-t}+c_2\e^t \\
  y(0) &= 0 = c_1+c_2 \\
  y &= c_1\e^{-t}-c_1\e^t \\
  y' &= -c_1\e^{-t}-c_1\e^t \\
  y'(\pi) &= 1 = -c_1\e^{-\pi}-c_1\e^{\pi} \\
  &= c_1(-\e^{-\pi}-\e^{\pi}) \\
  c_1 &= \frac{1}{-\e^{-\pi}-\e^{\pi}} \\
  y &= \frac{\e^{-t}}{-\e^{-\pi}-\e^{\pi}}-\frac{\e^t}{-\e^{-\pi}-\e^{\pi}}
\end{align*}

\subsubsection*{Problem 2}

\begin{center}
  If you have any questions, comments, or concerns, please contact me at
  alvin@omgimanerd.tech
\end{center}

\end{document}
