\documentclass[letterpaper, 12pt]{math}

\usepackage{amsmath}
\usepackage{amssymb}

\title{Series}
\author{Alvin Lin}
\date{Calculus II: August 2016 - December 2016}

\begin{document}

\maketitle

\section*{Series}
Sequence \( \bigg\{a_{1},...a_{n},...\bigg\} \equiv \bigg\{a_{n}\bigg\} \).
\[ \sum{a_{n}} = a_{1}+a_{2}+a_{3}+...+a_{n}+... = S_{n} \]
\begin{align*}
  \mathrm{If:} & \quad \lim_{n\to\infty}{S_{n}} = S \\
  \mathrm{Then:} & \quad \sum{a_{n}} \mathrm{\ converges},
    \quad \sum{a_{n}} = S, \quad \sum{a_{n}}<\infty
\end{align*}

\subsection*{Geometric Series}
\[ S_{n} = a+ar+ar^{2}+ar^{3}+... \]
\[ rS_{n} = ar+ar^{2}+ar^{3}+... \]
\[ S_{n}(1-r) = a-ar^{n} \]
\[ S_{n} = \frac{a(1-r^{n})}{1-r} \]
\[ \lim_{n\to\infty}{S_{n}} = \lim_{n\to\infty}{\frac{a(1-r^{n})}{1-r}} \]
\[ \lim_{n\to\infty}{S_{n}} = \frac{a}{1-r}; |r| < 1 \]
If \( \sum{a_{n}} \) converges, then \( \lim_{n\to\infty}{a_{n}} = 0 \). Proof:
\[ S_{n}-S_{n-1} = a_{n} \]
\[ \lim_{n\to\infty}{S_{n}-S_{n-1}} = \lim_{n\to\infty}{a_{n}} \]
\[ S-S = \lim_{n\to\infty}{a_{n}} = 0 \]

\subsection*{Problem 23}
\[ \sum_{k=2}^{\infty}\frac{k^{2}}{k^{2}-1} = \frac{4}{3}+\frac{9}{8}+...\]
\[ a_{n} = \frac{n^{2}}{n^{2}-1} \]
\[ \sum{a_{n}} = a_{1}+a_{1}r+a_{1}r^{2}+... \]
\[ \frac{a_{3}}{a_{2}} = \frac{a_{2}}{a_{1}} = r \]
\[ \sum{a_{n}} < \infty \]
\[ \lim_{n\to\infty}a_{n}\to1 \therefore \sum{a_{n}}\to\infty \quad
   \mathrm{(Diverging)} \]

\subsection*{Problem 25}
\[ \sum\frac{1+2^{n}}{2^{n}} \]
\begin{align*}
  \sum\frac{1+2^{n}}{2^{n}} &= \sum\frac{1}{3^{n}}+\sum\frac{2^{n}}{3^{n}} \\
  &= \sum(\frac{1}{3})^{n}+\sum(\frac{2}{3})^{n} \\
  &= \frac{a}{1-r}+\frac{a}{1-r} \\
  &= \frac{\frac{1}{3}}{1-\frac{1}{3}}+\frac{\frac{2}{3}}{1-\frac{2}{3}} \\
  &= \frac{1}{2}+\frac{2}{1} \\
  &= \frac{5}{2}
\end{align*}

\subsection*{Problem 29}
\[ \sum_{n=1}^{\infty}\ln(\frac{n^{2}+1}{2n^{2}+1}) \]
\[ a_{n} = \ln(\frac{n^{2}+1}{2n^{2}+1}) \]
\begin{align*}
  \lim_{n\to\infty}a_{n} &= \lim_{n\to\infty}\ln(\frac{n^{2}+1}{2n^{2}+1}) \\
  &= \lim_{n\to\infty}
    \ln(\frac{n^{2}(1+\frac{1}{n^{2}})}{n^{2}(2+\frac{1}{n^{2}})}) \\
  &= \lim_{n\to\infty}
    \ln(\frac{1+\frac{1}{n^{2}}}{2+\frac{1}{n^{2}}}) \\
  &= \ln(\frac{1}{2})
\end{align*}
\[ \lim_{n\to\infty}a_{n} = \ln(\frac{1}{2}) \therefore
   \sum{a_{n}} = \infty \quad \mathrm{(Diverges)} \]

\subsection*{Problem 33}
\[ \sum_{n=1}^{\infty}\bigg[\frac{1}{\e^{n}}+\frac{1}{n(n+1)}\bigg] \]
\[ \sum_{n=1}^{\infty}\bigg[\frac{1}{\e^{n}}+\frac{1}{n(n+1)}\bigg] =
   \sum_{n=1}^{\infty}\frac{1}{\e^{n}}+\sum_{n=1}^{\infty}\frac{1}{n(n+1)} \]
\begin{align*}
  \sum_{n=1}^{\infty}\frac{1}{\e^{n}} &=
    \frac{1}{\e}+\frac{1}{\e^{2}}+\frac{1}{\e^{3}}+... \\
  &= \frac{1}{1-r} \\
  &= \frac{\frac{1}{\e}}{1-\frac{1}{\e}} \\
  &= \frac{1}{\e-1} \\
  \sum_{n=1}^{\infty}\frac{1}{n(n+1)} &=
    \sum_{n=1}^{\infty}\frac{1}{n}-\frac{1}{n+1} \\
  &= (1-\frac{1}{2})+(\frac{1}{2}-\frac{1}{3})+(\frac{1}{3}-\frac{1}{4})+... \\
  &= 1 \\
  \sum_{n=1}^{\infty}\bigg[\frac{1}{\e^{n}}+\frac{1}{n(n+1)}\bigg] &=
    \frac{1}{\e-1}+1
\end{align*}

\subsection*{Problem 35}
\[ \sum_{n=2}^{\infty}\frac{2}{n^{2}-1} \]
\begin{align*}
  a_{n} &= \frac{2}{n^{2}-1} \\
  &= \frac{2}{(n-1)(n+1)} \\
  &= \frac{(n+1)-(n-1)}{(n-1)(n+1)} \\
  &= \frac{1}{n-1}-\frac{1}{n+1} \\
  \sum_{n=2}^{\infty}a_{n} &= \sum_{n=2}^{\infty}\frac{1}{n-1}-\frac{1}{n+1} \\
  &= (1-\frac{1}{3})+(\frac{1}{2}-\frac{1}{4})+(\frac{1}{3}-\frac{1}{5})+
    (\frac{1}{4}-\frac{1}{6})+... \\
  S_{n} &= (1-\frac{1}{3})+(\frac{1}{2}-\frac{1}{4})+...+
    (\frac{1}{n-1}-\frac{1}{n+1}) \\
  &= 1+\frac{1}{2}-\frac{1}{n-1}-\frac{1}{n} \\
  \lim_{n\to\infty}S_{n} &= \frac{3}{2}
\end{align*}

\begin{center}
  If any errors are found, please contact me at alvin.lin.dev@gmail.com
\end{center}

\end{document}
