\documentclass{math}

\title{The Comparison Tests}
\author{Alvin Lin}
\date{Calculus II: August 2016 - December 2016}

\begin{document}

\maketitle

\section*{The Comparison Tests}
If \( \sum{a_{n}} \) and \( \sum{b_{n}} \) are two series with positive entries:
\begin{enumerate}
  \item If \( \sum{b_{n}} \) converges and \( a_{n} \leq b_{n} \), then
    \( \sum{a_{n}} \) converges
  \item If \( \sum{a_{n}} \) diverges and \( a_{n} \leq b_{n} \), then
    \( \sum{b_{n}} \) diverges
  \item If \( \sum{b_{n}} \) diverges and \( b_{n} \leq a_{n} \), then
    \( \sum{a_{n}} \) diverges
\end{enumerate}

\subsection*{Example 1}
\[ \sum\frac{n}{2n^{3}+1} \]
\[ \frac{n}{2n^{3}+1} \leq \frac{n}{2n^{3}-1} = \frac{n}{2n^{3}} =
   \frac{1}{2n^{2}} \]
Integral test:
\begin{align*}
  \int_{1}^{\infty}\frac{1}{2x^{2}}\diff{x} &=
    \lim_{b\to\infty}\bigg[-\frac{x^{-1}}{2}\bigg]_{1}^{b} \\
  &= \lim_{b\to\infty}\bigg[-\frac{1}{2b}+\frac{1}{2}\bigg] \\
  &= \frac{1}{2} \quad \mathrm{(Convergent)}
\end{align*}
Therefore, since \( \sum\frac{n}{2n^{3}+1} \leq \sum\frac{1}{2n^{2}} \) and
\( \sum\frac{1}{2n^{2}} \) is convergent, \( \sum\frac{n}{2n^{3}+1} \) is
also convergent.

\subsection*{Example 2}
\[ \sum\frac{n+1}{n\sqrt{n}} \]
\[ \frac{n+1}{n\sqrt{n}} > \frac{n}{n\sqrt{n}} \]
\[ \frac{1}{\sqrt{n}} = \infty \quad \therefore \quad \sum\frac{n+1}{n\sqrt{n}}
   \quad \mathrm{diverges} \]

\subsection*{Example 3}
\[ \sum\frac{9^{n}}{3+10^{n}} \]
\[ \frac{9^{n}}{3+10^{n}} < \frac{9^{n}}{3+10^{n}-3} = (\frac{9}{10})^{n} \]
\[ \sum(\frac{9}{10})^{n} = \frac{a}{1-r} =
   \frac{\frac{9}{10}}{1-\frac{9}{10}} = 9 \]
\[ \sum(\frac{9}{10})^{n} \mathrm{converges} \quad \therefore \quad
   \sum\frac{9^{n}}{3+10^{n}} \quad \mathrm{diverges} \]

\subsection*{Practice Problem 4}
\[ \sum\frac{n^{3}}{n^{4}-1} \]
\[ \frac{n^{3}}{n^{4}-1} > \frac{n^{3}}{n^{4}} = \frac{1}{n} \]
\[ \frac{1}{n} = \infty \quad \therefore \quad \sum\frac{n^{3}}{n^{4}-1}
   \quad \mathrm{diverges} \]

\subsection*{Practice Problem 8}
\[ \sum\frac{4+3^{n}}{2^{n}} \]
\[ \frac{4+3^{n}}{2^{n}} > \frac{3^{n}}{2^{n}} \]
\[ \sum\frac{3^{n}}{2^{n}} = \infty \quad \therefore \quad
   \sum\frac{4+3^{n}}{2^{n}} \quad \mathrm{diverges} \]

\subsection*{Practice Problem 10}
\[ \sum\frac{n^{2}-1}{3n^{4}+1} \]
\[ \frac{n^{2}+1}{3n^{4}+1} < \frac{n^{2}}{3n^{4}+1} < \frac{n^{2}}{3n^{4}} =
   \frac{1}{3n^{2}} \]
\[ \sum\frac{1}{3n^{2}} < \infty \quad \therefore \quad
   \sum\frac{n^{2}-1}{3n^{4}+1} \quad \mathrm{converges} \]

\subsection*{Practice Problem 12}
\[ \sum\frac{1+\sin(n)}{10^{n}} \]
\[ \frac{1+\sin(n)}{10^{n}} \leq \frac{2}{10^{n}} \]
\[ \sum\frac{2}{10^{n}} = \frac{a}{1-r} < \infty
   \therefore \quad \sum\frac{1+\sin(n)}{10^{n}} \quad \mathrm{converges} \]

\subsection*{Practice Problem 13}
\[ \sum\frac{\arctan(n)}{n^{1.2}} \]
\[ \frac{\arctan(n)}{n^{1.2}} < \frac{\frac{\pi}{2}}{n^{1.2}} \]
\[ \sum\frac{\frac{\pi}{2}}{n^{1.2}} < \infty
   \therefore \quad \sum\frac{\arctan(n)}{n^{1.2}} \quad \mathrm{converges} \]

\subsection*{Practice Problem 14}
\[ \sum_{n=1}^{\infty}\frac{\sqrt{n^{3}+1}}{3n^{3}+4n^{2}+2} \]
\[ a_{n} = \frac{\sqrt{n^{3}+1}}{3n^{3}+4n^{2}+2} \]
\[ b_{n} = \frac{n^{\frac{3}{2}}}{3n^{3}} = \frac{1}{3n^{\frac{3}{2}}}
   \quad \mathrm{(converges)} \]
\begin{align*}
  \lim_{n\to\infty}\frac{a_{n}}{b_{n}} &=
    \frac{\frac{\sqrt{n^{3}+1}}{3n^{3}+4n^{2}+2}}
    {\frac{1}{3n^{\frac{3}{2}}}} \\
  &= \lim_{n\to\infty}\frac{3n^{3}}{3n^{3}+4n^{2}+2}
    \frac{\sqrt{n^{3}+1}}{\sqrt{n^{3}}} \\
  &= 1
\end{align*}
Therefore, \( \sum{a_{n}} \) converges (p-series test).

\subsection*{Practice Problem 15}
\[ \sum_{n=1}^{\infty}\frac{n-1}{2n+1} \]
\[ a_{n} = \frac{n-1}{2n+1} \]
\[ \lim_{n\to\infty}a_{n} = \frac{1}{2} \neq 0 \quad \therefore \quad
   \sum_{n=1}^{\infty}\frac{n-1}{2n+1} \quad \mathrm{diverges} \]

\begin{center}
  You can find all my notes at \url{http://omgimanerd.tech/notes}. If you have
  any questions, comments, or concerns, please contact me at
  alvin@omgimanerd.tech
\end{center}

\end{document}
