\documentclass[letterpaper, 12pt]{math}

\usepackage{tikz}
\usetikzlibrary{quotes,angles}

\geometry{letterpaper, margin=1in}

\title{Section 7.8}
\author{Alvin Lin}
\date{Calculus II: August 2016 - December 2016}

\begin{document}

\maketitle

\section*{Problem 5}
\[ \int_{3}^{\infty}{\frac{1}{(x-2)^{3/2}}\diff{x}} \]
\[ \lim_{b \to \infty}\int_{3}^{b}{(x-2)^{\frac{3}{2}}\diff{x}} \]
\[ Let: u = x-2 \]
\[ \diff{u} = \diff{x} \]
\[ \lim_{b \to \infty}\int_{3}^{b}{u^{\frac{3}{2}}\diff{u}} \]
\[ \lim_{b \to \infty}\bigg[\frac{-1}{2\sqrt{u}}\bigg]_{3}^{b} \]
\[ \lim_{b \to \infty}\bigg[\frac{-1}{2\sqrt{b}}-\frac{-1}{2\sqrt{3}}] \]
\[ = \frac{\sqrt{3}}{6} \]

\section*{Problem 7}
\[ \int_{-\infty}^{0}{\frac{1}{3-4x}\diff{x}} \]
\[ \lim_{b \to -\infty}\int_{b}^{0}{\frac{1}{3-4x}\diff{x}} \]
\[ Let: u = 3-4x \]
\[ \diff{u} = -4\diff{x} \]
\[ \frac{-1}{4}\lim_{b \to -\infty}\int_{b}^{0}{\frac{1}{u}\diff{u}} \]
\[ \frac{-1}{4}\lim_{b \to -\infty}\bigg[\ln|3-4x|\bigg]_{b}^{0} \]
\[ \frac{-1}{4}\lim_{b \to -\infty}\bigg[\ln|3|-\ln|3-4b|] \]
\[ = \infty \]

\section*{Problem 13}
\[ \int_{-\infty}^{\infty}{x\e^{-x^{2}}\diff{x}} \]
\[ \int_{-\infty}^{0}{x\e^{-x^{2}}\diff{x}}+
   \int_{0}^{\infty}{x\e^{-x^{2}}\diff{x}} \]
Solve as an indefinite integral:
\[ \int{x\e^{-x^{2}}\diff{x}} \]
\[ \frac{-1}{2}\int{-2x\e^{-x^{2}}\diff{x}} \]
\[ e^{-x^{2}}+C \]
Substitute the original limits:
\[ -\frac{1}{2}\lim_{a \to -\infty}\bigg[\e^{-x^{2}}\bigg]_{a}^{0}-
   \frac{1}{2}\lim_{b \to \infty}\bigg[\e^{-x^{2}}\bigg]_{0}^{b} \]
\[ -\frac{1}{2}\lim_{a \to -\infty}\bigg[\e^{-a^{2}}-\e^{0}\bigg]-
   \frac{1}{2}\lim_{b \to \infty}\bigg[\e^{0}-\e^{-b^{2}}\bigg] \]
\[ = 0 \]

\section*{Problem 29}
\[ \int_{-2}^{14}{(x+2)^{-1/4}\diff{x}} \]
Solve as an indefinite integral:
\[ \int{(x+2)^{-1/4}\diff{x}} \]
\[ Let: f'(x) = x^{-1/4}\diff{x} \quad g(x) = x+2 \]
\[ f(x) = \frac{4}{3}x^{3/4} \quad g'(x) = \diff{x} \]
\[ f(g(x)) = \frac{4}{3}(x+2)^{3/4} \]
Substitute the original limits:
\[ \frac{4}{3}\bigg[(x+2)^{3/4}\bigg]_{-2}^{14} \]
\[ \frac{4}{3}\bigg[(14+2)^{3/4}-(-2+2)^{3/4}\bigg] \]
\[ \frac{4}{3}\bigg[(14+2)^{3/4}-(-2+2)^{3/4}\bigg] \]
\[ \frac{4}{3}\bigg[8-0\bigg] \]
\[ = \frac{32}{3} \]

\section*{Problem 33}
\[ \int_{0}^{9}{\frac{1}{\sqrt[3]{x-1}}\diff{x}} \]
Solve as an indefinite integral:
\[ \int{\frac{1}{\sqrt[3]{x-1}}\diff{x}} \]
\[ Let: u = x-1 \]
\[ \diff{u} = \diff{x} \]
\[ \int{u^{-2/3}\diff{u}} \]
\[ 3u^{1/3}+C \]
\[ 3(x-1)^{1/3}+C \]
Substitute the original limits:
\[ 3\bigg[(x-1)^{1/3}\bigg]_{0}^{9} \]
\[ 3\bigg[\sqrt[3]{0}-\sqrt[3]{8}] \]
\[ = -6 \]

\begin{center}
  If you have any questions, comments, or concerns, please contact me at
  alvin@omgimanerd.tech
\end{center}

\end{document}
