\documentclass{math}

\geometry{letterpaper, margin=1in}

\title{Section 8.2}
\author{Alvin Lin}
\date{Calculus II: August 2016 - December 2016}

\begin{document}

\maketitle

\section*{Section 8.2}

\subsection*{Exercise 6}
\[ y = \arctan(x) \quad \quad 0 \leq x \leq 2 \]
\[ \frac{\diff{y}}{\diff{x}} = \frac{1}{1+x^{2}} \]
Rotated about the x-axis:
\begin{align*}
  S &= \int{(2\pi y)\diff{S}} \\
  &= 2\pi\int_{0}^{2}{y\sqrt{1+(\frac{\diff{y}}{\diff{x}})^{2}}\diff{x}} \\
  &= 2\pi\int_{0}^{2}{\arctan(x)\sqrt{1+(\frac{1}{1+x^{2}})^{2}}\diff{x}} \\
  & \approx 9.79564
\end{align*}
Rotated about the y-axis:
\begin{align*}
  S &= 2\pi\int_{0}^{2}{x\sqrt{1+(\frac{\diff{y}}{\diff{x}})^{2}}\diff{x}} \\
  & \approx 13.721
\end{align*}

\subsection*{Exercise 12}
\[ y = \frac{x^{3}}{6}+\frac{1}{2x} \quad \quad \frac{1}{2} \leq x \leq 1 \]
\[ y = \frac{x^{3}}{6}+\frac{1}{2x} = \frac{x^{4}+3}{6x} \]
\[ \frac{\diff{y}}{\diff{x}} = \frac{x^{4}-1}{2x^{2}} \]
Rotated about the x-axis:
\begin{align*}
  S &= \int(2\pi y)\diff{S} \\
  &= 2\pi\int_{\frac{1}{2}}^{1}{
    y\sqrt{1+(\frac{\diff{y}}{\diff{x}})^{2}}\diff{x}} \\
  &= 2\pi\int_{\frac{1}{2}}^{1}{(\frac{x^{4}+3}{6x})
    \sqrt{1+(\frac{x^{4}-1}{2x^{2}})^{2}}\diff{x}} \\
  &= 2\pi\int_{\frac{1}{2}}^{1}{(\frac{x^{4}+3}{6x})
    \sqrt{1+\frac{x^{8}-2x^{4}+1}{4x^{4}}}\diff{x}} \\
  &= 2\pi\int_{\frac{1}{2}}^{1}{(\frac{x^{4}+3}{6x})
    \sqrt{\frac{x^{8}-2x^{4}+4x^{4}+1}{4x^{4}}}\diff{x}} \\
  &= 2\pi\int_{\frac{1}{2}}^{1}{(\frac{x^{4}+3}{6x})
    \sqrt{\frac{x^{8}+2x^{4}+1}{4x^{4}}}\diff{x}} \\
  &= 2\pi\int_{\frac{1}{2}}^{1}{(\frac{x^{4}+3}{6x})
    \sqrt{\bigg(\frac{x^{4}+1}{2x^{2}}\bigg)^{2}\diff{x}}} \\
  &= 2\pi\int_{\frac{1}{2}}^{1}{(\frac{x^{4}+3}{6x})
    \frac{x^{4}+1}{2x^{2}}\diff{x}} \\
  &= 2\pi\int_{\frac{1}{2}}^{2}{\frac{x^{8}+4x^{4}+3}{12x^{3}}\diff{x}} \\
  &= 2\pi\int_{\frac{1}{2}}^{2}{
    \frac{x^{8}}{12x^{3}}+\frac{4x^{4}}{12x^{3}}+\frac{3}{12x^{3}}\diff{x}} \\
  &= 2\pi\int_{\frac{1}{2}}^{2}{
    \frac{x^{5}}{12}+\frac{x}{3}+\frac{1}{4x^{3}}\diff{x}} \\
  &= 2\pi\bigg[\frac{x^{6}}{72}+\frac{x^{2}}{6}-\frac{1}{8x^{2}}\bigg]
    _{\frac{1}{2}}^{1} \\
  &= \frac{263\pi}{256}
\end{align*}

\subsection*{Exercise 14}
\[ x = 1+2y^{2} \quad 1 \leq y \leq 2 \]
\[ \frac{\diff{x}}{\diff{y}} = 4y \]
Rotated about the x-axis:
\begin{align*}
  S &= \int(2\pi y)\diff{S} \\
  &= 2\pi\int_{1}^{2}{ y\sqrt{1+(\frac{\diff{x}}{\diff{y}})^{2}}\diff{x}} \\
  &= 2\pi\int_{1}^{2}{y\sqrt{1+(4y)^{2}}\diff{y}} \\
  &= 2\pi\int_{1}^{2}{y\sqrt{1+16y^{2}}\diff{y}} \\
  & Let: \quad u = 1+16y^{2} \quad \diff{u} = 32y\diff{y} \\
  &= 2\pi\int{y\sqrt{u}\frac{\diff{u}}{32y}} \\
  &= \frac{\pi}{16}\int{\sqrt{u}\diff{u}} \\
  &= \frac{\pi}{16}\frac{2u^{\frac{3}{2}}}{3} \\
  &= \frac{\pi}{24}\bigg[(1+8y^{2})^{\frac{3}{2}}\bigg]_{\frac{1}{2}}^{1} \\
  & \approx 59.42
\end{align*}

\subsection*{Exercise 17}
\[ x = \sqrt{a^{2}-y^{2}} \quad 0 \leq y \leq \frac{a}{2} \]
\[ \frac{\diff{x}}{\diff{y}} = \frac{1}{2}(a^{2}-y^{2})^{-\frac{1}{2}}(-2y)
   = \frac{-y}{\sqrt{a^{2}-y^{2}}} \]
Rotated about the y-axis:
\begin{align*}
  S &= \int{2\pi x\diff{S}} \\
  &= 2\pi\int_{0}^{a/2}{
    \sqrt{a^{2}-y^{2}}\sqrt{1+(\frac{\diff{x}}{\diff{y}})^{2}}\diff{x}} \\
  &= 2\pi\int_{0}^{a/2}{
    \sqrt{a^{2}-y^{2}}\sqrt{1+(\frac{-y}{\sqrt{a^{2}-y^{2}}})^{2}}\diff{x}} \\
  &= 2\pi\int_{0}^{a/2}{
    \sqrt{a^{2}-y^{2}}\sqrt{1+\frac{y^{2}}{a^{2}-y^{2}}}\diff{x}} \\
  &= 2\pi\int_{0}^{a/2}{
    \sqrt{a^{2}-y^{2}}\sqrt{\frac{a^{2}-y^{2}+y^{2}}{a^{2}-y^{2}}}\diff{x}} \\
  &= 2\pi\int_{0}^{a/2}{
    \sqrt{a^{2}-y^{2}}\sqrt{\frac{a^{2}}{a^{2}-y^{2}}}\diff{x}} \\
  &= 2\pi\int_{0}^{a/2}{
    \sqrt{a^{2}-y^{2}}\frac{\sqrt{a^{2}}}{\sqrt{a^{2}-y^{2}}}\diff{y}} \\
  &= 2\pi\int_{0}^{a/2}{2\pi a\diff{y}} \\
  &= 2\pi a\bigg[y\bigg]_{0}^{a/2} \\
  &= 2\pi a(\frac{a}{2}) \\
  &= \pi a^{2}
\end{align*}

\subsection*{Exercise 19}
\[ y = \frac{x^{5}}{5} \quad \quad 0 \leq x \leq 5 \]
\[ \frac{\diff{x}}{\diff{y}} = x^{4} \]
Rotated about the x-axis:
\begin{align*}
  S &= \int{2\pi y\diff{S}} \\
  &= 2\pi\int_{0}^{5}{
    \frac{x^{5}}{5}\sqrt{1+(\frac{\diff{x}}{\diff{y}})^{2}}\diff{x}} \\
  &= 2\pi\int_{0}^{5}{\frac{x^{5}}{5}\sqrt{1+(x^{4})^{2}}\diff{x}} \\
  &= \frac{2\pi}{5}\int_{0}^{5}{x^{5}\sqrt{1+x^{8}}\diff{x}} \\
\end{align*}
Using Simpson's Rule with n = 10:
\[ S \approx \frac{2\pi}{5} \times 979206.52 \approx 1230506.16 \]

\subsection*{Exercise 22}
\[ y = x\ln(x) \quad \quad 1 \leq x \leq 2 \]
\[ \frac{\diff{y}}{\diff{x}} = 1+\ln(x) \]
Rotated about the x-axis:
\begin{align*}
  S &= \int{2\pi y\diff{S}} \\
  &= 2\pi\int_{0}^{2}{x\ln(x)\sqrt{1+(1+\ln(x))^{2}}\diff{x}} \\
  &= 2\pi\int_{0}^{2}{x\ln(x)\sqrt{1+1+2\ln(x)+(\ln(x))^{2}}\diff{x}} \\
  &= 2\pi\int_{0}^{2}{x\ln(x)\sqrt{(\ln(x))^{2}+2\ln(x)+2}\diff{x}}
\end{align*}
Using Simpson's Rule with n = 10:
\[ S \approx 7.25 \]

\begin{center}
  If you have any questions, comments, or concerns, please contact me at
  alvin@omgimanerd.tech
\end{center}

\end{document}
