\documentclass[letterpaper, 12pt]{math}

\geometry{letterpaper, margin=1in}

\title{Section 11.1}
\author{Alvin Lin}
\date{Calculus II: August 2016 - December 2016}

\begin{document}

\maketitle

\section*{Problem 9}
\[ a_{1} = 1 \quad a_{n+1} = 5a_{n}-3 \]
\begin{align*}
  a_{2} &= 5(1)-3 = 2 \\
  a_{3} &= 5(2)-3 = 7 \\
  a_{4} &= 5(7)-3 = 32 \\
  a_{5} &= 5(32)-3 = 157
\end{align*}

\section*{Problem 17}
Given:
\[ \bigg\{\frac{1}{2},-\frac{4}{3},
   \frac{9}{4},-\frac{16}{5},\frac{25}{6}\bigg\} \]
Find \( a_{n} \):
\[ a_{n} = \frac{n^{2}(-1)^{n+1}}{n+1} \]

\section*{Problem 25}
\[ a_{n} = \frac{n^{4}}{n^{3}-2n} \]
\begin{align*}
  \lim_{n\to\infty}{a_{n}} &= \lim_{n\to\infty}{\frac{n^{4}}{n^{3}-2n}} \\
  &= \lim_{n\to\infty}{\frac{n^{4}}{n^{3}-2n}
    \frac{\frac{1}{n^{3}}}{\frac{1}{n^{3}}}} \\
  &= \lim_{n\to\infty}{\frac{n}{1-\frac{2}{n^{2}}}} \\
  &= \infty
\end{align*}
This sequence is divergent.

\section*{Problem 29}
\[ a_{n} = \e^{\frac{-1}{\sqrt{n}}} \]
\begin{align*}
  \lim_{n\to\infty}{a_{n}} &= \lim_{n\to\infty}{\e^{\frac{-1}{\sqrt{n}}}} \\
  &= \e^{0} \\
  &= 1
\end{align*}

\section*{Problem 33}
\[ a_{n} = \cos(\frac{n}{2}) \]
\[ \lim_{n\to\infty}{a_{n}} = \cos(\infty) = \mathrm{undefined} \]
This sequence is divergent.

\section*{Problem 36}
\[ a_{n} = \frac{(-1)^{n+1}n}{n+\sqrt{n}} \]
\[ \lim_{n\to\infty}{|a_{n}|} = \lim_{n\to\infty}{\frac{n}{n+\sqrt{n}}} = 1 \]
\begin{center}
  Since \( \lim_{n\to\infty}{|a_{n}|} \neq 0 \),
  \( \lim_{n\to\infty}{a_{n}} \neq 0 \), (Theorem). \\
  Therefore, this sequence is divergent.
\end{center}

\begin{center}
  If you have any questions, comments, or concerns, please contact me at
  alvin@omgimanerd.tech
\end{center}

\end{document}
